Add unreadable

src/prop/MemoryProps.v
@@ -1616,6 +1616,87 @@ Section UNCHANGABLES.
       eapply x1; eauto.
   Qed.
 
+  Inductive unreadable (mem prom: Memory.t) (l: Loc.t) (t: Time.t): Prop :=
+  | unreadable_intro
+      (UNWRITABLE: unwritable mem prom l t)
+      (NOTCONCRETE: forall
+          from val released
+          (GET: Memory.get l t mem = Some (from, Message.concrete val released)), False)
+  .
+
+  Lemma unreadable_increase pf e lang (th0 th1: Thread.t lang)
+        (STEP: Thread.step pf e th0 th1)
+    :
+      unreadable th0.(Thread.memory) th0.(Thread.local).(Local.promises) <2=
+      unreadable th1.(Thread.memory) th1.(Thread.local).(Local.promises).
+  Proof.
+    ii. inv PR. inv UNWRITABLE.
+    dup UNCH. eapply unchangable_increase in UNCH; eauto. split.
+    { econs; eauto. }
+    { ii. inv UNCH. exploit Memory.get_disjoint.
+      { eapply GET. }
+      { eapply GET0. }
+      i. des.
+      { subst. eapply NOTCONCRETE; eauto.
+        inv UNCH0. eauto. }
+      { eapply x2; eauto. econs; ss; [|refl].
+        eapply memory_get_ts_strong in GET. des; auto.
+        subst. inv ITV. ss. inv FROM. }
+    }
+  Qed.
+
+  Lemma rtc_unreadable_increase lang (th0 th1: Thread.t lang)
+        (STEP: rtc (Thread.tau_step (lang:=lang)) th0 th1)
+    :
+      unreadable th0.(Thread.memory) th0.(Thread.local).(Local.promises) <2=
+      unreadable th1.(Thread.memory) th1.(Thread.local).(Local.promises).
+  Proof.
+    induction STEP; eauto.
+    i. inv H. inv TSTEP. eapply IHSTEP. eapply unreadable_increase; eauto.
+  Qed.
+
+  Lemma step_no_read_unreadable lang (th_tgt th_tgt': Thread.t lang) e_tgt pf
+        (STEP: Thread.step pf e_tgt th_tgt th_tgt')
+    :
+      no_read_msgs (unreadable th_tgt.(Thread.memory) th_tgt.(Thread.local).(Local.promises))
+                   e_tgt.
+  Proof.
+    inv STEP.
+    - inv STEP0; ss.
+    - inv STEP0; ss. inv LOCAL; ss.
+      + ii. inv H. inv LOCAL0. eapply NOTCONCRETE; eauto.
+      + ii. inv H. inv LOCAL1. eapply NOTCONCRETE; eauto.
+  Qed.
+
+  Lemma steps_no_read_unreadable P lang (th_tgt th_tgt': Thread.t lang)
+        (STEP: rtc (tau (@pred_step P lang)) th_tgt th_tgt')
+    :
+      rtc (tau (@pred_step (P /1\ no_read_msgs (unreadable th_tgt.(Thread.memory) th_tgt.(Thread.local).(Local.promises))) lang)) th_tgt th_tgt'.
+  Proof.
+    ginduction STEP.
+    - i. refl.
+    - i. inv H. inv TSTEP. econs 2.
+      + econs; eauto. econs; eauto.
+        split; auto. inv STEP0. eapply step_no_read_unreadable; eauto.
+      + inv STEP0. eapply pred_step_rtc_mon; eauto.
+        i. ss. des. split; auto. eapply no_read_msgs_mon; eauto.
+        i. eapply unreadable_increase; eauto.
+  Qed.
+
+  Lemma no_read_unreadable_traced lang (th0 th1: Thread.t lang) tr
+        (STEPS: traced_step tr th0 th1)
+    :
+      List.Forall (fun em => (no_read_msgs (unreadable th0.(Thread.memory) th0.(Thread.local).(Local.promises))) (fst em)) tr.
+  Proof.
+    ginduction STEPS.
+    - econs.
+    - subst. inv HD. econs.
+      + ss. eapply step_no_read_unreadable in STEP; eauto.
+      + eapply List.Forall_impl; eauto. i. ss.
+        eapply no_read_msgs_mon; eauto.
+        i. eapply unreadable_increase; eauto.
+  Qed.
+
 End UNCHANGABLES.
 
 
